instantiated quotientfilter

Structures/QuotientFilter/QuotientFilter_Definitions.v
@@ -17,8 +17,12 @@ Unset Printing Implicit Defensive.
 From ProbHash.Computation
      Require Import Comp Notationv1.
 
+From ProbHash.Utils
+     Require Import InvMisc seq_ext.
+
+
 From ProbHash.Core
-     Require Import Hash HashVec FixedList.
+     Require Import Hash HashVec FixedList AMQ AMQHash.
 
 
 Module Type QuotientFilterSpec.
@@ -31,10 +35,6 @@ Module Type QuotientFilterSpec.
    r - the number of elements in the remainder - 1
   *)
   Parameter  r:nat.
-  (*
-   n - maximum number of elements a single fingerprint can hold
-  *)
-  Parameter  n:nat.
 
   (* type being hashed in the quotient filter *)
   Parameter  B:finType.
@@ -75,7 +75,7 @@ Module QuotientFilterDefinitions (Spec: QuotientFilterSpec).
   Qed.
   
 
-  Record QuotientFilter := mkQuotientFilter
+  Record QuotientFilter (n: nat) := mkQuotientFilter 
                              {
                                quotientfilter_state:
                                (* maps each quotient value *)
@@ -84,49 +84,49 @@ Module QuotientFilterDefinitions (Spec: QuotientFilterSpec).
                                        (fixlist [eqType of 'I_r.+1] n.+1)
                              }.
   
-  Definition Quotientfilter_prod (bf: QuotientFilter) :=
+  Definition Quotientfilter_prod (n: nat) (bf: QuotientFilter n) :=
     (quotientfilter_state bf).
 
-  Definition prod_Quotientfilter  pair := let: (state) := pair in @ mkQuotientFilter state.
+  Definition prod_Quotientfilter (n:nat) pair := let: (state) := pair in @ mkQuotientFilter n state.
 
-  Lemma quotientfilter_cancel : cancel (Quotientfilter_prod) (prod_Quotientfilter).
+  Lemma quotientfilter_cancel n : cancel (@Quotientfilter_prod n) (@prod_Quotientfilter n).
   Proof.
       by case.
   Qed.
 
-  Definition quotientfilter_eqMixin :=
-    CanEqMixin quotientfilter_cancel .
+  Definition quotientfilter_eqMixin n :=
+    CanEqMixin (@quotientfilter_cancel n) .
 
-  Canonical quotientfilter_eqType  :=
-    Eval hnf in EqType QuotientFilter  quotientfilter_eqMixin .
+  Canonical quotientfilter_eqType n  :=
+    Eval hnf in EqType (QuotientFilter n)  (quotientfilter_eqMixin n) .
 
-  Definition quotientfilter_choiceMixin :=
-    CanChoiceMixin quotientfilter_cancel.
+  Definition quotientfilter_choiceMixin n:=
+    CanChoiceMixin (@quotientfilter_cancel n).
 
-  Canonical quotientfilter_choiceType  :=
-    Eval hnf in ChoiceType QuotientFilter  quotientfilter_choiceMixin.
+  Canonical quotientfilter_choiceType n  :=
+    Eval hnf in ChoiceType (QuotientFilter n)  (@quotientfilter_choiceMixin n).
 
-  Definition quotientfilter_countMixin :=
-    CanCountMixin quotientfilter_cancel.
+  Definition quotientfilter_countMixin n :=
+    CanCountMixin (@quotientfilter_cancel n).
 
-  Canonical quotientfilter_countType :=
-    Eval hnf in CountType QuotientFilter  quotientfilter_countMixin.
+  Canonical quotientfilter_countType n :=
+    Eval hnf in CountType (QuotientFilter n)  (@quotientfilter_countMixin n).
 
-  Definition quotientfilter_finMixin :=
-    CanFinMixin quotientfilter_cancel .
+  Definition quotientfilter_finMixin n :=
+    CanFinMixin (@quotientfilter_cancel n).
 
-  Canonical quotientfilter_finType :=
-    Eval hnf in FinType QuotientFilter  quotientfilter_finMixin.
+  Canonical quotientfilter_finType n :=
+    Eval hnf in FinType (QuotientFilter n)  (@quotientfilter_finMixin n).
 
 
-  Definition quotientfilter_new : QuotientFilter :=
-    mkQuotientFilter (nseq_tuple q.+1 (fixlist_empty [eqType of 'I_r.+1] n.+1)).
+    Definition quotientfilter_new n : QuotientFilter n :=
+      mkQuotientFilter (nseq_tuple q.+1 (fixlist_empty [eqType of 'I_r.+1] n.+1)).
 
-  Lemma quotient_num_quotient (value: 'I_(q.+1 * r.+1)) : (value %% q.+1 < q.+1).
-  Proof.
-    move: value => [m Hm] //=.
-    by apply ltn_pmod.
-  Qed.
+    Lemma quotient_num_quotient (value: 'I_(q.+1 * r.+1)) : (value %% q.+1 < q.+1).
+    Proof.
+      move: value => [m Hm] //=.
+        by apply ltn_pmod.
+    Qed.
   
   Lemma quotient_num_remainder (value: 'I_(q.+1 * r.+1)) : (value %/ q.+1 < r.+1).
   Proof.
@@ -152,35 +152,23 @@ Module QuotientFilterDefinitions (Spec: QuotientFilterSpec).
   Qed.
 
 
-  
-  Definition quotientfilter_add_internal (value: 'I_(q.+1 * r.+1)) qf : QuotientFilter :=
+  Section Definitions.
+
+    Variable n: nat.
+
+  Definition quotientfilter_add_internal (value: 'I_(q.+1 * r.+1)) qf : QuotientFilter n:=
     let: (quotient,remainder) := quotient_num value in
     let quotient_list := tnth (quotientfilter_state qf) quotient in
     let quotient_list' := fixlist_insert quotient_list remainder in
     mkQuotientFilter
       (set_tnth (quotientfilter_state qf) quotient_list' quotient).
-
-
-  Definition quotientfilter_add (value: hash_keytype) (hashes: HashState n) (qf: QuotientFilter) :
-    Comp [finType of HashState n * QuotientFilter ] :=
-    hash_res <-$ (@hash _ value hashes);
-      let (new_hashes, hash_vec) := hash_res in
-      let qres := quotientfilter_add_internal (hash_value_coerce hash_vec) qf in
-      ret (new_hashes, qres).
-
-  Definition quotientfilter_add_multiple  hsh_0 bf_0 values :=
-    @foldr _ (Comp [finType of  HashState n * QuotientFilter])
-           (fun val hsh_bf =>
-              res_1 <-$ hsh_bf;
-                let (hsh, bf) := res_1 in
-                quotientfilter_add val hsh bf) (ret (hsh_0, bf_0)) values.
   
   Definition quotientfilter_query_internal (value: 'I_(q.+1 * r.+1)) qf : bool :=
     let: (quotient,remainder) := quotient_num value in
-    let quotient_list := tnth (quotientfilter_state qf) quotient in
+    let quotient_list := tnth (@quotientfilter_state n qf) quotient in
     fixlist_contains remainder quotient_list.
 
-  Definition quotientfilter_query (value: hash_keytype) (hashes: HashState n) (qf: QuotientFilter) :
+  Definition quotientfilter_query (value: hash_keytype) (hashes: HashState n) (qf: QuotientFilter n) :
     Comp [finType of HashState n * bool ] :=
     hash_res <-$ (@hash _ value hashes);
       let (new_hashes, hash_vec) := hash_res in
@@ -188,10 +176,10 @@ Module QuotientFilterDefinitions (Spec: QuotientFilterSpec).
       ret (new_hashes, qres).
 
   Definition quotientfilter_has_free_spaces l qf :=
-    all (fun ls => [length ls] + l <= n ) (quotientfilter_state qf).
+    all (fun ls => [length ls] + l <= n ) (@quotientfilter_state n qf).
 
   Definition quotientfilter_valid  qf :=
-    all (fun ls => fixlist_is_top_heavy ls) (quotientfilter_state qf).
+    all (fun ls => fixlist_is_top_heavy ls) (@quotientfilter_state n qf).
 
   Lemma fixlist_length_empty (A:eqType) k :
         [length (fixlist_empty A k)] = 0.
@@ -199,15 +187,17 @@ Module QuotientFilterDefinitions (Spec: QuotientFilterSpec).
     rewrite/fixlist_length/fixlist_empty/fixlist_unwrap //=.
     elim: k => [//=|k IHk //=].
   Qed.
-  
+
+  End Definitions.
     
   Section Theorems.
 
     Variable l: nat.
+    Variable n: nat.
     Hypothesis Hl: l > 0.
 
     Lemma quotientfilter_new_free_spaces :
-      quotientfilter_has_free_spaces n (quotientfilter_new).
+      quotientfilter_has_free_spaces n (quotientfilter_new n).
     Proof.
       rewrite/quotientfilter_has_free_spaces/quotientfilter_new.
       apply/allP => ls; move=>/nseqP [Hls1 Hls2].
@@ -215,7 +205,7 @@ Module QuotientFilterDefinitions (Spec: QuotientFilterSpec).
     Qed.
 
     Lemma quotientfilter_new_valid :
-      quotientfilter_valid (quotientfilter_new).
+      quotientfilter_valid (quotientfilter_new n).
     Proof.
       rewrite/quotientfilter_has_free_spaces/quotientfilter_new.
       apply/allP => ls; move=>/nseqP [Hls1 Hls2].
@@ -228,7 +218,7 @@ Module QuotientFilterDefinitions (Spec: QuotientFilterSpec).
     Lemma quotientfilter_add_query_base qf value:
       quotientfilter_valid qf ->
       quotientfilter_has_free_spaces l qf ->
-      quotientfilter_query_internal value (quotientfilter_add_internal value qf).
+      @quotientfilter_query_internal n value (quotientfilter_add_internal value qf).
     Proof.
       move: qf => [qf]//=; rewrite/quotientfilter_valid/quotientfilter_has_free_spaces
       => /allP Hvalid  /allP //=  Hall.
@@ -244,7 +234,7 @@ Module QuotientFilterDefinitions (Spec: QuotientFilterSpec).
       quotientfilter_valid qf ->
       quotientfilter_has_free_spaces l qf ->
       qf' = (quotientfilter_add_internal value qf) ->
-      quotientfilter_valid qf' && quotientfilter_has_free_spaces l.-1 qf'.
+      quotientfilter_valid qf' && @quotientfilter_has_free_spaces n l.-1 qf'.
     Proof.
       move: qf qf' => [qf] //= [qf']//=; rewrite/quotientfilter_valid/quotientfilter_has_free_spaces
       => /allP Hvalid /allP Hall.
@@ -269,7 +259,7 @@ Module QuotientFilterDefinitions (Spec: QuotientFilterSpec).
 
     Lemma quotientfilter_add_query_preserve qf value value' :
       quotientfilter_query_internal value qf ->
-      quotientfilter_query_internal value (quotientfilter_add_internal value' qf).
+      @quotientfilter_query_internal n value (quotientfilter_add_internal value' qf).
     Proof.
       move: qf => [qf].
       rewrite /quotientfilter_query_internal; move: (quotient_num value) => [quotient remainder].
@@ -293,7 +283,7 @@ Module QuotientFilterDefinitions (Spec: QuotientFilterSpec).
     
     Lemma quotientfilter_add_query_eq qf value value' :
       ~~ quotientfilter_query_internal value qf ->
-      quotientfilter_query_internal value (quotientfilter_add_internal value' qf) ->
+      @quotientfilter_query_internal n value (quotientfilter_add_internal value' qf) ->
       value = value'.
     Proof.
       rewrite /quotientfilter_query_internal.
@@ -322,7 +312,140 @@ Module QuotientFilterDefinitions (Spec: QuotientFilterSpec).
 
     End Theorems.
 
+
+
 End QuotientFilterDefinitions.
+
+Module QuotientFilterAMQ (Spec: QuotientFilterSpec).
+
+  Module QuotientFilterDefinitions :=  QuotientFilterDefinitions Spec.
+  Module BasicHash := AMQHash.BasicHash QuotientFilterDefinitions.QuotientHash.
+
+  Export BasicHash.
+  Export QuotientFilterDefinitions.
+
+  Module AMQ <: AMQ BasicHash.
+
+      Definition AMQStateParams := nat.
+      Definition AMQState (n: AMQStateParams) : finType :=
+        [finType of QuotientFilter n].
+
+      Section AMQ.
+        Variable p: AMQStateParams.
+        Variable h: BasicHash.AMQHashParams.
+
+        Definition AMQ_add_internal
+                   (amq: AMQState p) (value: BasicHash.AMQHashValue h):
+          AMQState p := quotientfilter_add_internal value amq.
+        
+        Definition AMQ_query_internal
+                   (amq: AMQState p) (key: BasicHash.AMQHashValue h) : bool :=
+          quotientfilter_query_internal key amq.
+
+        Definition AMQ_available_capacity
+                   (h: BasicHash.AMQHashParams) (amq: AMQState p) (l:nat): bool:=
+          quotientfilter_has_free_spaces (h.+1 * l) amq.
+
+        Definition AMQ_valid (amq:AMQState p) : bool :=
+          quotientfilter_valid amq.
+
+        Definition AMQ_new: AMQState p := quotientfilter_new p.
+
+        Lemma AMQ_new_nqueryE: forall vals, ~~ AMQ_query_internal  AMQ_new vals.
+        Proof.
+          move=> vals; rewrite/AMQ_query_internal/quotientfilter_query_internal//=.
+          rewrite tnth_nseq_eq.
+          rewrite/fixlist_contains //=.
+          apply/hasPn => v.
+          move: (@fixlist_empty_is_empty [eqType of 'I_r.+1] p.+1).
+          rewrite/fixlist_is_empty =>/eqP -> //=.
+        Qed.
+        
+        Lemma AMQ_new_validT: AMQ_valid AMQ_new.
+        Proof.
+            by apply quotientfilter_new_valid.
+        Qed.
+        
+        Section DeterministicProperties.
+          Variable amq: AMQState p.
+
+          Lemma AMQ_available_capacityW: forall  n m,
+              AMQ_valid amq -> m <= n -> AMQ_available_capacity h amq n -> AMQ_available_capacity h amq m.
+          Proof.
+            move=> n m Hvalid Hnm /allP Hvv; apply/allP => v Hv; move:(Hvv v Hv) => //=.
+            apply leq_trans; rewrite leq_add2l //=.
+              by rewrite leq_mul2l Hnm; apply/orP; right.
+          Qed.
+        End DeterministicProperties.
+
+        Section DeterministicProperties.
+          Variable amq: AMQState p.
+
+          Lemma AMQ_add_query_base: forall (amq: AMQState p) inds,
+              AMQ_valid amq -> AMQ_available_capacity h amq 1 ->
+              AMQ_query_internal (AMQ_add_internal amq inds) inds.
+          Proof.
+            apply quotientfilter_add_query_base.
+          Qed.
+          
+          Lemma AMQ_add_valid_preserve: forall (amq: AMQState p) inds,
+              AMQ_valid amq -> AMQ_available_capacity h amq 1 ->
+              AMQ_valid (AMQ_add_internal amq inds).
+          Proof.
+            rewrite /AMQ_available_capacity muln1/AMQHashValue/AMQ_valid.
+            rewrite/quotientfilter_valid/quotientfilter_has_free_spaces.
+            move=> [amq'] ind /allP Hvv /allP Hspace; apply /allP => v.
+            rewrite/AMQ_add_internal/quotientfilter_add_internal.
+            case_eq (quotient_num ind) => quot rem Heq.
+
+            have H f:  quotientfilter_state {|  quotientfilter_state := f |} = f; first by [].
+            rewrite !H.
+            move=>/tnthP [ quot' ].
+            case Hquot: (quot' != quot).
+            - rewrite tnth_set_nth_neq; first move=>->; last by [].
+              apply Hvv.
+                by apply mem_tnth.
+            - move/Bool.negb_true_iff: Hquot; rewrite Bool.negb_involutive => /eqP ->.
+              rewrite tnth_set_nth_eq; first move=>->; last by [].
+              apply fixlist_insert_preserves_top_heavy.
+              apply Hvv.
+                by apply mem_tnth.
+          Qed.
+
+          Lemma AMQ_add_query_preserve: forall (amq: AMQState p) inds inds',
+              AMQ_valid amq -> AMQ_available_capacity h amq 1 -> AMQ_query_internal amq inds ->
+              AMQ_query_internal (AMQ_add_internal amq inds') inds.
+          Proof.
+            move=> amq' ind inds' Hvalid Hcap.
+              by apply quotientfilter_add_query_preserve.
+          Qed.
+          
+          Lemma AMQ_add_capacity_decr: forall (amq: AMQState p) inds l,
+              AMQ_valid amq -> AMQ_available_capacity h amq l.+1 ->
+              AMQ_available_capacity h (AMQ_add_internal amq inds) l.
+          Proof.
+            move=> amq' ind l Hvalid Hcap.
+            rewrite /AMQ_available_capacity in Hcap.
+            have Hobv: 0 < h.+1 * l.+1; first by rewrite muln_gt0; apply/andP;split => //=.
+            move: (@quotientfilter_add_preserve
+                     _ p Hobv amq'
+                     (quotientfilter_add_internal ind amq')
+                     ind Hvalid Hcap
+                     (Logic.eq_refl
+                        (quotientfilter_add_internal ind amq'))
+                  ) => /andP [_ ].
+
+            rewrite/AMQ_available_capacity.
+            rewrite mulnS addnC addnS -pred_Sn.
+            move=>/allP Hvv; apply/allP => v Hv; move: (Hvv v Hv).
+              by rewrite addnA =>/leq_addr_weaken.
+          Qed.
+
+        End DeterministicProperties.
+      End AMQ.
+    End AMQ.  
+End QuotientFilterAMQ.
+
 
 
 
