Structures/QuotientFilter/QuotientFilter_Probability.v
@@ -30,34 +30,48 @@ From ProbHash.QuotientFilter
 
 
 
+Module QuotientFilterProperties (Spec:  QuotientFilterSpec).
 
+  Module QuotientFilterCore :=  (QuotientFilterAMQ Spec).
+  Module QuotientFilterDefinitions :=  QuotientFilterCore.QuotientFilterDefinitions.
+  Module BasicHash :=  QuotientFilterCore.BasicHash.
+  Module QuotientFilterAMQ :=  QuotientFilterCore.AMQ.
+  Module QuotientFilterOperations :=  AMQ.AMQOperations (BasicHash)  (QuotientFilterAMQ).
 
-
-Module QuotientFilterProbability (Spec:  QuotientFilterSpec).
-  Module QuotientFilterDefinitions := (QuotientFilterDefinitions Spec).
+  Export BasicHash.
   Export QuotientFilterDefinitions.
+  Export QuotientFilterOperations.
+
+  Section Theorems.
+
+    Variable n: nat.
+    Variable k: nat.
 
   Lemma quotientfilter_add_multiple_find_preserve values l m hshs hshs' qf qf' ind value
         (Huniq: uniq (value :: values))
         (Hlen: length values == l) 
-        (Hfree: hash_has_free_spaces  ((l+m).+1)  hshs)
-        (Huns:      all (fun val => hash_unseen val hshs) values)
-        (Hcontains:  hashstate_find n value hshs == Some ind)
-    : ((d[ @quotientfilter_add_multiple hshs qf values]) (hshs', qf') != (0 %R)) ->
-      (hash_has_free_spaces  (m.+1) hshs') && (hashstate_find n value hshs' == Some ind).
+        (Hfree: AMQHash_hashstate_available_capacity  hshs  ((l+m).+1))
+        (Huns:      all (fun val => AMQHash_hashstate_unseen hshs val) values)
+        (Hcontains:  AMQHash_hashstate_find hshs value == Some ind)
+    : ((d[ @AMQ_add_multiple k n hshs qf values]) (hshs', qf') != (0 %R)) ->
+      (AMQHash_hashstate_available_capacity  hshs' (m.+1)) && (@AMQHash_hashstate_find k hshs' value == Some ind).
   Proof.
     (* First clean up the proof *)
-    move=> //=.
+    move: hshs hshs' qf qf'  ind values value Hlen Huniq Hfree Huns Hcontains.
+    rewrite/AMQ_add_multiple/AMQHashKey/AMQ_add/AMQHash_hash/AMQ_add_internal/AMQHash_hashstate_available_capacity/AMQHash_hashstate_find/AMQHash/AMQState/AMQHashValue/AMQHashKey/AMQHash_hashstate_unseen //=.
+    move=> hshs hshs' qf qf'  ind values value Hlen Huniq Hfree Huns Hcontains.
+    (* move=> //=. *)
     move: m hshs Hfree Huns qf qf' hshs' Hcontains.
     move/eqP: Hlen <-; clear l.
-    rewrite/hashes_have_free_spaces/hash_has_free_spaces/hashes_value_unseen/hash_unseen.
+    rewrite/AMQHash_hashstate_available_capacity.
     (* proof has been cleaned up *)
     elim: values Huniq => [//= Huniq | y ys IHy Huniq] m hshs Hfree Huns qf qf' hshs' Hcontains.
     - {
-        comp_normalize => /bool_neq0_true; rewrite xpair_eqE => /andP[/eqP -> _]; rewrite Hcontains Bool.andb_true_r.
+        comp_normalize => /bool_neq0_true.
+        move=>/eqP/pair_equal_spec [-> _].
+        rewrite Hcontains Bool.andb_true_r.
           by move: Hfree; rewrite add0n.
       }
-
     - {
         comp_normalize.
         exchange_big_outwards 2; comp_simplify_n 1.
@@ -65,36 +79,39 @@ Module QuotientFilterProbability (Spec:  QuotientFilterSpec).
         move=>   n_hshs' n_qf' n_ind' Haddm Hhash /bool_neq0_true/eqP Hqf.
         have Huniq': (uniq (value :: ys)); first
           by move: Huniq => //=; rewrite in_cons Bool.negb_orb => /andP[/andP[_ ->]/andP[_ ->]].
-        move: Hfree => //=; rewrite -addnS addSn => Hfree.
+        move: Hfree => //=.
+        rewrite -(addnS (length ys).+1 m) addSn.
+        move=> Hfree.
         move: Huns => //= /andP [Hfun Hall].
         move: (IHy Huniq' m.+1 hshs Hfree Hall qf  n_qf' n_hshs' Hcontains Haddm) => /andP [Hlen Hfind].
-
-
-        move: Hhash; rewrite /hash; case: (hashstate_find n y n_hshs') => [n_ind'' | ] //=.
+        move: Hhash; rewrite /Hash.hash; case: (Hash.hashstate_find k y n_hshs') => [n_ind'' | ] //=.
         - comp_normalize => /bool_neq0_true; rewrite xpair_eqE => /andP[/eqP -> _]; rewrite Hfind Bool.andb_true_r.
             by move: Hlen; rewrite addnS =>/ltnW.
         - comp_normalize; comp_simplify.
           under eq_bigr do rewrite eq_sym xpair_eqE andbC boolR_distr -mulRA; comp_simplify.
           rewrite mulR_neq0' => /andP[/bool_neq0_true /eqP <- _].
           apply/andP; split; rewrite/hashstate_find/hashstate_put.
-            by apply fixedlist_add_incr; move: Hlen; rewrite addnS.
-
-            have Hvalneq: (value != y); first by move: Huniq => //=; rewrite in_cons Bool.negb_orb => /andP[/andP[]].
-            rewrite /hashstate_find in Hfind.
-              by apply fixmap_find_eq.
+          rewrite /Hash.hashstate_put/fixlist_length .
+          by move:  (@fixedlist_add_incr _ _ _ m.+2 k n_hshs' n_ind' y Hlen); rewrite addnS.
+          have Hvalneq: (value != y); first by move: Huniq => //=; rewrite in_cons Bool.negb_orb => /andP[/andP[]].
+          rewrite /Hash.hashstate_find in Hfind.
+            by apply fixmap_find_eq.
       }
-
   Qed.
-  
+
+
   Lemma quotientfilter_add_multiple_find_preserve_alt values l m hshs hshs' qf qf' ind value
         (Huniq: uniq (value :: values))
         (Hlen: length values == l) 
         (Hfree: hash_has_free_spaces  ((l+m))  hshs)
-        (Huns:      all (fun val => hash_unseen val hshs) values)
-        (Hcontains:  hashstate_find n value hshs == Some ind)
-    : ((d[ @quotientfilter_add_multiple hshs qf values]) (hshs', qf') != (0 %R)) ->
-      (hashstate_find n value hshs' == Some ind).
+        (Huns:      all (fun val => AMQHash_hashstate_unseen hshs val) values)
+        (Hcontains:  @AMQHash_hashstate_find k hshs value == Some ind)
+    : ((d[ @AMQ_add_multiple k n hshs qf values]) (hshs', qf') != (0 %R)) ->
+      (AMQHash_hashstate_find hshs' value == Some ind).
   Proof.
+    move: values hshs hshs' qf qf' ind value Huniq Hlen Hfree Huns Hcontains.
+    rewrite/AMQ_add_multiple/AMQHashKey/AMQ_add/AMQHash_hash/AMQ_add_internal/AMQHash_hashstate_available_capacity/AMQHash_hashstate_find/AMQHash/AMQState/AMQHashValue/AMQHashKey/AMQHash_hashstate_unseen //=.
+    move=> values hshs hshs' qf qf' ind value Huniq Hlen Hfree Huns Hcontains.
     (* First clean up the proof *)
     move=> //=.
     move: m hshs Hfree Huns qf qf' hshs' Hcontains.
@@ -116,7 +133,7 @@ Module QuotientFilterProbability (Spec:  QuotientFilterSpec).
 
         move: Hfree => //=  ; rewrite addSn -addnS => Hfree.
         move: (IHy Huniq' m.+1 hshs Hfree Hall qf  n_qf' n_hshs' Hcontains Haddm).
-        move: Hhash; rewrite /hash; case: (hashstate_find n y n_hshs') => [n_ind'' | ] //=.
+        move: Hhash; rewrite /Hash.hash; case: (Hash.hashstate_find k y n_hshs') => [n_ind'' | ] //=.
         - by comp_normalize => /bool_neq0_true; rewrite xpair_eqE => /andP[/eqP -> _].
         - comp_normalize; comp_simplify.
           under eq_bigr do rewrite eq_sym xpair_eqE andbC boolR_distr -mulRA; comp_simplify.
@@ -130,10 +147,13 @@ Module QuotientFilterProbability (Spec:  QuotientFilterSpec).
 
   Lemma quotientfilter_add_multiple_find_neq_preserve values hshs hshs' qf qf' value
         (Huniq: uniq (value :: values))
-        (Hcontains:  hashstate_find n value hshs == None)
-    : ((d[ @quotientfilter_add_multiple hshs qf values]) (hshs', qf') != (0 %R)) ->
-      (hashstate_find n value hshs' == None).
+        (Hcontains:  AMQHash_hashstate_find hshs value == None)
+    : ((d[ @AMQ_add_multiple k n hshs qf values]) (hshs', qf') != (0 %R)) ->
+      (Hash.hashstate_find k value hshs' == None).
   Proof.
+    move: values hshs hshs' qf qf' value Huniq Hcontains.
+    rewrite/AMQ_add_multiple/AMQHashKey/AMQ_add/AMQHash_hash/AMQ_add_internal/AMQHash_hashstate_available_capacity/AMQHash_hashstate_find/AMQHash/AMQState/AMQHashValue/AMQHashKey/AMQHash_hashstate_unseen //=.
+    move=> values hshs hshs' qf qf' value Huniq Hcontains.
     elim:  values qf qf' hshs hshs' Hcontains Huniq => [//=| x xs Hxs] qf qf' hshs hshs' Hcontains Huniq.
     - by comp_normalize => /bool_neq0_true; rewrite xpair_eqE=>/andP[/eqP -> _]; rewrite Hcontains.
     - move: Huniq => //= /andP[];rewrite in_cons Bool.negb_orb=>/andP[Hneq Hnin] /andP[Hninxs Huniqxs].
@@ -144,8 +164,8 @@ Module QuotientFilterProbability (Spec:  QuotientFilterSpec).
 
       have H1: uniq (value :: xs); first by move=> //=; rewrite Hnin Huniqxs.
       move: Hhash (Hxs qf qf'' hshs hshs'' Hcontains H1 Haddm) ; clear H1 Hxs.
-      rewrite/hash; case: (hashstate_find n x hshs'') => [v|] //=; comp_normalize.
-        by move=> /bool_neq0_true; rewrite xpair_eqE =>/andP[/eqP ->] //=.
+      rewrite/Hash.hash; case: (Hash.hashstate_find k x hshs'') => [v|] //=; comp_normalize.
+        - by move=> /bool_neq0_true; rewrite xpair_eqE =>/andP[/eqP ->] //=.
         comp_simplify; comp_possible_decompose => ind /bool_neq0_true; rewrite xpair_eqE => /andP[/eqP -> _] _.
         rewrite/hashstate_find/hashstate_put.
           by apply fixmap_find_neq.
@@ -153,9 +173,9 @@ Module QuotientFilterProbability (Spec:  QuotientFilterSpec).
 
 
   Lemma quotientfilter_add_mutliple_query_preserve qf qf' v hashes xs hshs':
-    (quotientfilter_query_internal v qf) ->
-    ((d[ quotientfilter_add_multiple hashes qf xs]) (hshs', qf')) != 0 ->
-    (quotientfilter_query_internal v qf').
+    (AMQ_query_internal qf v) ->
+    ((d[ @AMQ_add_multiple k n hashes qf xs]) (hshs', qf')) != 0 ->
+    (@AMQ_query_internal n k qf' v).
    Proof.
      elim: xs qf qf' hashes hshs' => [| x xs IHxs] qf qf' hashes hshs' Hqint//=; comp_normalize.
      - by move=>/bool_neq0_true; rewrite xpair_eqE =>/andP [_ /eqP ->].
@@ -164,19 +184,20 @@ Module QuotientFilterProbability (Spec:  QuotientFilterSpec).
        apply/quotientfilter_add_query_preserve.
        by apply (IHxs _ _ _ _ Hqint Hi1) => //=.
    Qed.
-   
        
 
 
   Lemma quotientfilter_add_multiple_properties_preserve values l m qf qf' hshs hshs'
         (Huniq: uniq values)
         (Hlen: length values == l) 
-        (Hfree: quotientfilter_has_free_spaces  ((l+m))  qf)
+        (Hfree: @quotientfilter_has_free_spaces n ((l+m))  qf)
         (Hvalid:   quotientfilter_valid qf)
-    : ((d[ @quotientfilter_add_multiple hshs qf values]) (hshs', qf') != (0 %R)) ->
-      quotientfilter_valid qf' &&  quotientfilter_has_free_spaces m qf'.
+    : ((d[ @AMQ_add_multiple k n hshs qf values]) (hshs', qf') != (0 %R)) ->
+      AMQ_valid qf' &&  quotientfilter_has_free_spaces m qf'.
   Proof.
-
+    move: values qf qf' hshs hshs' Huniq Hlen Hfree Hvalid.
+    rewrite/AMQ_add_multiple/AMQHashKey/AMQ_add/AMQHash_hash/AMQ_add_internal/AMQHash_hashstate_available_capacity/AMQHash_hashstate_find/AMQHash/AMQState/AMQHashValue/AMQHashKey/AMQHash_hashstate_unseen/AMQ_valid/AMQ_available_capacity //=.
+    move=> values qf qf' hshs hshs' Huniq Hlen Hfree Hvalid.
     move/eqP:Hlen Hfree => <-; clear l => Hfree .
     elim:  values m qf qf' hshs hshs'  Hvalid Hfree Huniq => [//=| x xs Hxs] m qf qf' hshs hshs' Hvalid Hfree Huniq.
     - by comp_normalize => /bool_neq0_true; rewrite xpair_eqE=>/andP[_ /eqP ->]; rewrite Hvalid //=.
@@ -190,27 +211,33 @@ Module QuotientFilterProbability (Spec:  QuotientFilterSpec).
       have H2: uniq xs; first by move: Huniq => //= /andP[].
       move: (Hxs m.+1 qf qf'' hshs hshs'' Hvalid H1 H2 Haddm) => /andP [Hvalid' Hfree']; clear H1 H2.
       have H1: (0 < m.+1); first by [].
-      move: (@quotientfilter_add_preserve m.+1 H1 qf'' qf' (hash_value_coerce value') Hvalid' Hfree' Hqf) => //=.
+      move: (@QuotientFilterDefinitions.quotientfilter_add_preserve  m.+1 n H1 qf'' qf' value' Hvalid' Hfree' Hqf) => //=.
   Qed.
   
+
   Theorem quotientfilter_no_false_negatives l hashes qf  x xs :
-    quotientfilter_valid qf  ->  quotientfilter_has_free_spaces l.+1 qf ->
-    uniq (x :: xs) -> length xs == l -> hash_has_free_spaces (l.+1) hashes  ->
-    all (fun x => hash_unseen x hashes) (x::xs) ->
-    (d[ res1 <-$ quotientfilter_add x hashes qf;
+    AMQ_valid qf  ->  AMQ_available_capacity n qf l.+1 ->
+    uniq (x :: xs) -> length xs == l -> AMQHash_hashstate_available_capacity hashes (l.+1)  ->
+    all (fun x => AMQHash_hashstate_unseen hashes x) (x::xs) ->
+    (d[ res1 <-$ AMQ_add qf hashes x;
           let '(hsh1, bf1) := res1 in
-          res2 <-$ quotientfilter_add_multiple hsh1 bf1 xs;
+          res2 <-$ @AMQ_add_multiple _ n hsh1 bf1 xs;
             let '(hsh2, bf2) := res2 in
-            res3 <-$ quotientfilter_query x hsh2 bf2;
+            res3 <-$ @AMQ_query k n bf2 hsh2 x;
               ret (snd res3) ] true) = (1 %R).
   Proof.
+    (* First clean up the proof *)
+    move: l hashes qf x xs.
+    rewrite/AMQ_add_multiple/AMQ_query/AMQ_query_internal/AMQ_available_capacity/AMQ_valid/AMQHashKey/AMQ_add/AMQHash_hash/AMQ_add_internal/AMQHash_hashstate_available_capacity/AMQHash_hashstate_find/AMQHash/AMQState/AMQHashValue/AMQHashKey/AMQHash_hashstate_unseen.
+    move=> l hashes qf x xs.
     (* elim: xs x cbf => [ | x' xs' Hxs'] x cbf *)
+
     move=> Hvalid Hcap Huniq Hlen Hfree Huns //=; comp_normalize.
     comp_simplify_n 2.
     exchange_big_outwards 5 => //=; comp_simplify_n 1.
     exchange_big_outwards 4 => //=; comp_simplify_n 1.
     move: Huns => //=/andP[/eqP Hunsx Hunsxs].
-    rewrite{1}/hash {1}/hashstate_find Hunsx; comp_normalize.
+    rewrite{1}/Hash.hash Hunsx; comp_normalize.
     exchange_big_outwards 2 => //=; comp_simplify_n 1.
     exchange_big_outwards 2 => //=; comp_simplify_n 1.
     exchange_big_outwards 4 => //=; comp_simplify_n 1.
@@ -218,9 +245,11 @@ Module QuotientFilterProbability (Spec:  QuotientFilterSpec).
     under_all ltac:(rewrite -!mulRA).
     case Hllen: (l == 0).
     - move/eqP: Hllen Hlen => ->; case: xs Huniq Hunsxs => [//=|//=] Huniq Hunsxs; move=> Hllen; comp_normalize.
-      comp_simplify; rewrite/hash; move: Hfree; rewrite/hash_has_free_spaces addnS -addSn -ltnS => /addr_ltn.
-      rewrite -[[length hashes].+1]addn1 ltnS => H.
-      under eq_bigr do under eq_bigr do under eq_bigr => i1 _ do rewrite (hash_find_insert_involutive _ _ _ _ H).
+      comp_simplify.
+      rewrite/Hash.hash; move: Hfree.
+      rewrite addnS -addSn => /addr_ltn.
+      rewrite -[[length hashes].+1]addn1 => /ltnW H.
+      under eq_bigr do under eq_bigr do under eq_bigr => i1 _ do rewrite (Hash.hash_find_insert_involutive _ _ _ _ H).
       comp_normalize; comp_simplify.
       under eq_bigr => i _ do rewrite (quotientfilter_add_query_base _ Hvalid Hcap) //= mul1R.
         by rewrite bigsum_card_constE mulRV //= card_ord RIneq.INR_IZR_INZ; apply/eqP => //=.
@@ -229,15 +258,19 @@ Module QuotientFilterProbability (Spec:  QuotientFilterSpec).
         => ind'' _; first under eq_rsum_ne0 => hsh' Hhsh.
         move/quotientfilter_add_multiple_find_preserve_alt: Hhsh => Hhsh.
         move: Hfree (Hfree) (Hhsh l 0 ind'' x Huniq Hlen) ; clear Hhsh; rewrite/hash_has_free_spaces/hashstate_put addn0.
-        rewrite addnS; move=>/fixedlist_add_incr =>/(_ ind'' x) => Hlength Hfree Hshs.
-        have Huns':  all ((hash_unseen (n:=n))^~ (fixmap_put x ind'' hashes)) xs. {
+        move=>/(@fixedlist_add_incr _ _ ) =>/(_ ind'' x) => Hlength Hfree Hshs.
+        have Huns':  all ((hash_unseen (n:=k))^~ (fixmap_put x ind'' hashes)) xs. {
           apply/allP => v Hv; move: Huniq => //=/andP[/memPn /(_ v Hv)] => Hneq _ .
             by move/allP: Hunsxs => /(_ v Hv)/(fixmap_find_neq) => /(_ x ind'' Hneq).
         }
-        have Hlen': [length hashes] + 1 <= n; first
+        have Hlen': [length hashes] + 1 <= k; first
                                                                                     by move/eqP: Hllen Hfree; clear; case: l => //= l _; rewrite addnS -addSn => /addr_ltn/ltnW; rewrite addn1.
-        move/eqP: (@hash_find_insert_involutive _ x ind'' hashes Hlen') => Hfind'; rewrite/hash.
-        move/eqP: (Hshs Hlength Huns' Hfind') -> => //=.
+        move/eqP: (@hash_find_insert_involutive _ x ind'' hashes Hlen') => Hfind'; rewrite/Hash.hash.
+        move: Hshs; rewrite/AMQHash_hashstate_available_capacity/Hash.hashstate_put=>Hshs.
+        have Hlength': length [unwrap fixmap_put x ind'' hashes] + l <= k;
+          first by move: Hlength; rewrite addnS =>/ltnW.
+        move/eqP: (Hshs Hlength' Huns' Hfind').
+        rewrite/AMQHash_hashstate_find =>-> //=.
           by over. by over. by over. by over. by over.
       }
       comp_normalize.
@@ -245,10 +278,12 @@ Module QuotientFilterProbability (Spec:  QuotientFilterSpec).
       exchange_big_outwards 1 => //=; comp_simplify_n 1.           
       under eq_bigr => qf' _. {
         under eq_bigr => inds' _; first under eq_rsum_ne0 => hshs' /quotientfilter_add_mutliple_query_preserve Hneq.
+        rewrite/AMQ_query_internal in Hneq.
         rewrite Hneq //=; first rewrite mul1R; first by over.
         apply (@quotientfilter_add_query_base l) => //=.
         move: Hcap; rewrite/quotientfilter_has_free_spaces =>/allP Hall; apply/allP => v Hv; move: (Hall v Hv).
-        by rewrite addnS => /ltnW.
+        by rewrite mulSn addnA => /leq_addr_weaken; rewrite addnS =>/ ltnW.
+        (* by rewrite addnS => /ltnW. *)
         by over. by over.
       }
       rewrite exchange_big //=; under eq_bigr => inds' _ . {
@@ -259,25 +294,26 @@ Module QuotientFilterProbability (Spec:  QuotientFilterSpec).
       }
       by rewrite bigsum_card_constE mulRV //= card_ord RIneq.INR_IZR_INZ; apply/eqP => //=.
   Qed.
-  
-
 
   Theorem quotientfilter_collision_prob hashes l value (values: seq B):
     l < n ->
     length values == l ->
-    hash_has_free_spaces (l.+1) hashes  ->
-    all (fun val => hash_unseen val hashes) (value::values) ->
+    AMQHash_hashstate_available_capacity hashes (l.+1)  ->
+    all (fun val => AMQHash_hashstate_unseen hashes val) (value::values) ->
     uniq (value::values) ->
     d[
-        res1 <-$ quotientfilter_query value hashes (quotientfilter_new);
+        res1 <-$ @AMQ_query k n (quotientfilter_new n) hashes value;
           let (hashes1, init_query_res) := res1 in
-          res2 <-$ @quotientfilter_add_multiple hashes1 (quotientfilter_new) values;
+          res2 <-$ @AMQ_add_multiple k n hashes1 (quotientfilter_new n) values;
             let (hashes2, bf) := res2 in
-            res' <-$ quotientfilter_query value hashes2 bf;
+            res' <-$ AMQ_query bf hashes2 value;
               ret (res'.2)
       ] true =
     (1 -R- (( 1 -R- Rdefinitions.Rinv (Hash_size.+1)) ^R^ l)).
   Proof.
+    move: l hashes value values.
+    rewrite/AMQ_add_multiple/AMQ_query/AMQ_query_internal/AMQ_available_capacity/AMQ_valid/AMQHashKey/AMQ_add/AMQHash_hash/AMQ_add_internal/AMQHash_hashstate_available_capacity/AMQHash_hashstate_find/AMQHash/AMQState/AMQHashValue/AMQHashKey/AMQHash_hashstate_unseen.
+    move=> l hashes value values.
     move=> Hln Hlen Hfree /allP Hall Huniq.
     comp_normalize.
     comp_simplify_n 2.
@@ -285,7 +321,7 @@ Module QuotientFilterProbability (Spec:  QuotientFilterSpec).
     exchange_big_outwards 4 => //=; comp_simplify_n 1.
     have Hin: (value \in value :: values); first by rewrite in_cons eq_refl //=.
     move: (@Hall _ Hin).
-    rewrite {1}/hash/hashstate_find/hash_unseen =>/eqP ->; comp_normalize.
+    rewrite {1}/Hash.hash/Hash.hashstate_find/hash_unseen =>/eqP ->; comp_normalize.
     exchange_big_outwards 2 => //=; comp_simplify_n 1.
     exchange_big_outwards 2 => //=; comp_simplify_n 1.
     exchange_big_outwards 4 => //=; comp_simplify_n 1.
@@ -299,45 +335,55 @@ Module QuotientFilterProbability (Spec:  QuotientFilterSpec).
       under eq_bigr do rewrite -!mulRA.
       under eq_rsum_ne0 => qf' Hqf.
       have Hhashlen:
-        hash_has_free_spaces (l + 0) (hashstate_put n value ind' hashes); first
-        by rewrite addn0; move: Hfree; rewrite/hash_has_free_spaces/hashstate_put addnS;
-        move=> /(@fixedlist_add_incr _ _ _ _ _ _ ind' value).
+        hash_has_free_spaces (l + 0) (Hash.hashstate_put k value ind' hashes). {
+         rewrite addn0; move: Hfree; rewrite/hash_has_free_spaces/Hash.hashstate_put.
+        by move=>/(@fixedlist_add_incr _ _ _ l.+1 k _ ind' value); rewrite addnS =>/ltnW.
+      }
       have Hhashall:
-        all ((hash_unseen (n:=n))^~ (hashstate_put n value ind' hashes)) values; first
+        all ((hash_unseen (n:=k))^~ (hashstate_put k value ind' hashes)) values; first
         by apply/allP => v Hvin; move/allP: Hall =>
       //=/andP[_ /allP Hall]; move: (Hall v Hvin);
         rewrite/hash_unseen/hashstate_put; apply fixmap_find_neq;
           move: Huniq => //=/andP[/memPn Hnin _]; move:(Hnin v Hvin).
       have Hhashfind:
-        hashstate_find n value (hashstate_put n value ind' hashes) == Some ind'; first
-        by rewrite hash_find_insert_involutive //=; move: Hfree;rewrite/hash_has_free_spaces addnS -addSn ;
-        move=> /InvMisc.addr_ltn; rewrite addn1.
+        Hash.hashstate_find k value (Hash.hashstate_put k value ind' hashes) == Some ind'. {
+        rewrite Hash.hash_find_insert_involutive //=; move: Hfree;rewrite/hash_has_free_spaces addnS -addSn ;
+          move=> /InvMisc.addr_ltn; rewrite addn1.
+        by rewrite -addn1 => /leq_addr_weaken.
+      }
       move: (@quotientfilter_add_multiple_find_preserve_alt
-               values l 0 (hashstate_put n value ind' hashes)
-               hshs' quotientfilter_new qf' ind' value Huniq Hlen
+               values l 0 (hashstate_put k value ind' hashes)
+               hshs' (quotientfilter_new n) qf' ind' value Huniq Hlen
                Hhashlen Hhashall Hhashfind Hqf
             ).
-      rewrite/hash => /eqP -> //=; rewrite FDist1.dE.
+      rewrite/AMQHash_hashstate_find/Hash.hash => /eqP -> //=; rewrite FDist1.dE.
         by over. by over. by over. by over. by over.
     }
     move=> //=; comp_simplify_n 2.
     under_all ltac:(rewrite  mulRA mulRC).
     under eq_bigr do (under eq_bigr do rewrite -rsum_Rmul_distr_l;  rewrite -rsum_Rmul_distr_l).
     suff H i:
-      \sum_(a in hashstate_of_finType n)
-       \sum_(a0 in quotientfilter_finType)
-       ((d[ quotientfilter_add_multiple (hashstate_put n value i hashes) quotientfilter_new values])
-          (a, a0) *R* (quotientfilter_query_internal (hash_value_coerce i) a0 %R)) =
+      \sum_(a in hashstate_of_finType k)
+       \sum_(a0 in quotientfilter_finType n)
+       ((d[ @AMQ_add_multiple k n (Hash.hashstate_put k value i hashes) (quotientfilter_new n) values])
+          (a, a0) *R* (quotientfilter_query_internal i a0 %R)) =
       (1 -R- ((1 -R- Rdefinitions.Rinv (Hash_size.+1)) ^R^ l)).
-    under eq_bigr do rewrite H.
+    rewrite/AMQ_add_multiple/AMQ_add/AMQHash/AMQState in H.
+    under eq_bigr => i Hi. {
+      move: (H i).
+      rewrite/hashstate_of_finType/AMQHashKey/AMQHash_hash/AMQ_add_internal/HashState/fixmap/fixlist //=.
+      move=>->.
+      by over.
+    } 
     rewrite bigsum_card_constE mulRA mulRV //= ?mul1R //= card_ord -add1n; apply/eqP; apply RIneq.not_0_INR => //=. 
     under_all ltac:(rewrite mulRC); under eq_bigr do rewrite -rsum_pred_demote; rewrite exchange_big //=.
-    move: (@rsum_pred_inv [finType of QuotientFilter]
-                          ((d[ res <-$ quotientfilter_add_multiple
-                                   (hashstate_put n value i hashes)
-                                   quotientfilter_new values;
+    move: (@rsum_pred_inv [finType of QuotientFilter n]
+                          ((d[ res <-$ @AMQ_add_multiple k n
+                                   (hashstate_put k value i hashes)
+                                   (quotientfilter_new n) values;
                                ret res.2 ]))
-                          (fun j => quotientfilter_query_internal (hash_value_coerce i) j)).
+                          (fun j => quotientfilter_query_internal i j)).
+    rewrite/AMQ_add_multiple/AMQ_add/AMQ_add_internal/AMQHash_hash //=.
     comp_normalize.
     under_all ltac:(rewrite mulRC eq_sym); under eq_bigr do under eq_bigr do rewrite -rsum_pred_demote big_pred1_eq.
     move=> ->; apply f_equal.
@@ -350,7 +396,7 @@ Module QuotientFilterProbability (Spec:  QuotientFilterSpec).
     - intros; comp_normalize; under_all ltac:(rewrite xpair_eqE boolR_distr -!mulRA);
         under eq_bigr do rewrite -rsum_pred_demote big_pred1_eq.
       rewrite -rsum_pred_demote big_pred1_eq.
-      suff ->: (quotientfilter_query_internal (hash_value_coerce i) quotientfilter_new = false); first by move=> //=.
+      suff ->: (@quotientfilter_query_internal n i (quotientfilter_new n) = false); first by move=> //=.
       apply Bool.negb_true_iff.
       rewrite/quotientfilter_query_internal/quotientfilter_new/fixlist_contains //=.
       apply/hasPn => x //=.
@@ -358,8 +404,9 @@ Module QuotientFilterProbability (Spec:  QuotientFilterSpec).
         by move: (fixlist_empty_is_empty [eqType of 'I_r.+1] n.+1); rewrite/fixlist_is_empty => /eqP -> //=.
     - move=> //= /andP [Huns Halluns ]; rewrite in_cons Bool.negb_orb => /andP[Hneq Hnin] /andP[/memPn Hyneq Huniq].
       move=> Hfree Hlen.
-      have Hfree': hash_has_free_spaces (length xs).+1 hashes; first
+      have Hfree': ([length hashes] + (length xs).+1 < k). {
         by move: Hfree; rewrite /hash_has_free_spaces; rewrite addnS =>/ltnW.
+      }
       have Hlen': length xs < n; first by move: Hlen => /ltnW.
       move: (IHxs Halluns Hnin Huniq Hfree' Hlen') => <-.
       comp_normalize.
@@ -372,18 +419,19 @@ Module QuotientFilterProbability (Spec:  QuotientFilterSpec).
       exchange_big_inwards ltac:(rewrite -rsum_Rmul_distr_l); rewrite -rsum_Rmul_distr_l.
       apply Logic.eq_sym.
       rewrite  mulRC -!mulRA.
-      case Haddm: ((d[ quotientfilter_add_multiple (hashstate_put n value i hashes) quotientfilter_new xs]) (hsh, qf) == 0);
+      case Haddm: ((d[ @AMQ_add_multiple k n (hashstate_put k value i hashes) (quotientfilter_new n) xs]) (hsh, qf) == 0);
         first by move/eqP: Haddm ->; rewrite !mul0R.
       move/Bool.negb_true_iff: Haddm => Haddm; apply f_equal.
       have H1: uniq (x :: xs); first by move=> //=; move/memPn: Hyneq => Hyneq; rewrite Hyneq Huniq.
-      have H2: hashstate_find n x (hashstate_put n value i hashes) == None; first
+      have H2: hashstate_find k x (hashstate_put k value i hashes) == None; first
         by move: Huns; rewrite/hash_unseen/hashstate_find; apply fixmap_find_neq; rewrite eq_sym.
       move: (@quotientfilter_add_multiple_find_neq_preserve
-               xs (hashstate_put n value i hashes) hsh
-               quotientfilter_new qf x
+               xs (hashstate_put k value i hashes) hsh
+               (quotientfilter_new n) qf x
                H1 H2 Haddm
             ); clear H1 H2 Hfree' Hlen'.
-      rewrite/hash =>/eqP ->; apply Logic.eq_sym.
+      rewrite/Hash.hash.
+      move=>/eqP ->; apply Logic.eq_sym.
       comp_normalize.
       under_all ltac:(rewrite mulRC -!mulRA xpair_eqE andbC boolR_distr -mulRA).
       exchange_big_inwards ltac:(rewrite -rsum_pred_demote big_pred1_eq).
@@ -392,27 +440,27 @@ Module QuotientFilterProbability (Spec:  QuotientFilterSpec).
       exchange_big_inwards ltac:(rewrite -rsum_pred_demote big_pred1_eq).
       rewrite (bigID (fun i0 => i0 == i)) big_pred1_eq //= addRC.
       have H1: (length xs == length xs); first by [].
-      have H2: (quotientfilter_has_free_spaces (length xs + (n - length xs)) quotientfilter_new); first
+      have H2: (quotientfilter_has_free_spaces (length xs + (n - length xs)) (quotientfilter_new n)); first
         by rewrite subnKC; first (by apply quotientfilter_new_free_spaces);
         move: Hlen; rewrite -addn1 => /addr_ltn/ltnW.
 
       move: (@quotientfilter_add_multiple_properties_preserve
-               xs  (length xs) (n - (length xs)) quotientfilter_new qf
-               (hashstate_put n value i hashes) hsh Huniq H1 H2 quotientfilter_new_valid Haddm
+               xs  (length xs) (n - (length xs)) (quotientfilter_new n) qf
+               (hashstate_put k value i hashes) hsh Huniq H1 H2 (quotientfilter_new_valid n) Haddm
             ) => /andP[ Hvalid' Hfree' ]; clear H1 H2.
       rewrite (@quotientfilter_add_query_base (n - length xs)); first rewrite  //= mulR0 //= addR0; try (by []); last first.
 
       have H i0: i0 != i ->
                  quotientfilter_query_internal
-                   (hash_value_coerce i) (quotientfilter_add_internal (hash_value_coerce i0) qf) = 
-                 quotientfilter_query_internal (hash_value_coerce i) qf.
+                   i (quotientfilter_add_internal i0 qf) = 
+                 quotientfilter_query_internal i qf.
       {
-        move=> Hi0; case Hquery : (quotientfilter_query_internal (hash_value_coerce i) qf).
-          by move: (@quotientfilter_add_query_preserve qf (hash_value_coerce i) (hash_value_coerce i0) Hquery) ->; move=> //=.
+        move=> Hi0; case Hquery : (quotientfilter_query_internal i qf).
+          by move: (@quotientfilter_add_query_preserve n qf i i0 Hquery) ->; move=> //=.
           move/Bool.negb_true_iff: Hquery => Hnequery.
           case Hquery : (quotientfilter_query_internal _ _) => //=.
-          move: (quotientfilter_add_query_eq Hnequery Hquery)=> Heq; move:  Heq Hi0.
-            by move=>/hash_value_coerce_eq -> /Bool.negb_true_iff; rewrite eq_refl => ->.
+          move: (quotientfilter_add_query_eq Hnequery Hquery)=> Heq; move:  Heq Hi0 => -> //=.
+          rewrite eq_refl //=.
       }
       under eq_bigr => i0 Hi0 do rewrite (@H i0 Hi0).
       rewrite -big_distrl //= mulRC; apply f_equal.
@@ -424,5 +472,74 @@ Module QuotientFilterProbability (Spec:  QuotientFilterSpec).
       under eq_bigl do rewrite Bool.negb_involutive; rewrite big_pred1_eq Uniform.dE card_ord//= .
         by do?(apply f_equal); rewrite RIneq.INR_IZR_INZ //=.
   Qed.
+
+  End Theorems.
   
-End QuotientFilterProbability.
+  Module QuotientFilterProperties <:  AMQ.AMQProperties (BasicHash) (QuotientFilterAMQ).
+    Module AmqOperations :=  QuotientFilterOperations.
+    Export AmqOperations.
+
+  
+    Definition AMQ_false_positive_probability (hash:  AMQHashParams) (state: AMQStateParams) (l: nat) : Rdefinitions.R := (1 -R- (( 1 -R- Rdefinitions.Rinv (Hash_size.+1)) ^R^ l)).
+
+    Section Properties.
+      Variable h : AMQHashParams.
+      Variable s: AMQStateParams.
+
+      Variable hashes: AMQHash h.
+
+      Section FalseNegatives.
+
+        Variable amq: AMQState s.
+
+        Lemma AMQ_no_false_negatives:
+          forall (l:nat_eqType) (x:AMQHashKey) (xs: seq AMQHashKey),
+            uniq (x :: xs) -> length xs == l ->
+
+            AMQ_valid amq -> AMQ_available_capacity h amq l.+1 ->
+
+            AMQHash_hashstate_valid hashes ->
+            AMQHash_hashstate_available_capacity hashes l.+1 ->
+            all (AMQHash_hashstate_unseen hashes) (x::xs) ->
+            (d[ res1 <-$ AMQ_add amq hashes x;
+                  let '(hsh1, amq1) := res1 in
+                  res2 <-$ AMQ_add_multiple hsh1 amq1 xs;
+                    let '(hsh2, amq2) := res2 in
+                    res3 <-$ AMQ_query amq2 hsh2 x;
+                      ret (snd res3) ] true) = (1 %R).
+        Proof.
+          apply AMQ_no_false_negatives.
+        Qed.
+
+      End FalseNegatives.
+
+      Theorem AMQ_false_positives_rate: forall  l value (values: seq _),
+          length values == l ->
+
+          AMQHash_hashstate_valid hashes ->
+          AMQHash_hashstate_available_capacity hashes (l.+1) ->
+
+
+          AMQ_available_capacity h (AMQ_new s) l.+1 ->
+          all (AMQHash_hashstate_unseen hashes) (value::values) ->
+          uniq (value::values) ->
+          d[ 
+              res1 <-$ AMQ_query (AMQ_new s) hashes value;
+                let (hashes1, init_query_res) := res1 in
+                res2 <-$ AMQ_add_multiple hashes1 (AMQ_new s) values;
+                  let (hashes2, amq) := res2 in
+                  res' <-$ AMQ_query amq  hashes2 value;
+                    ret (res'.2)
+            ] true = AMQ_false_positive_probability h s l.
+      Proof.
+        move=> l value values Hlen Hvalid Havail Hcap Hall Huniq.
+        rewrite (@quotientfilter_collision_prob s h hashes l value values) //=.
+        move: Hcap; rewrite/AMQ_available_capacity.
+        rewrite/QuotientFilterCore.QuotientFilterDefinitions.quotientfilter_has_free_spaces.
+        rewrite all_nseq //= addnC =>/leq_addr_weaken.
+        by rewrite mulSn=>/leq_addr_weaken.
+      Qed.
+    End Properties.
+  End QuotientFilterProperties.
+End QuotientFilterProperties.
+
